\begin{aligned} (1)\ & \left\{\begin{matrix} p(y=1|x;\theta)=h_\theta(x) \\ \ \ \ \ \ p(y=0|x;\theta)=1-h_\theta(x) \end{matrix}\right.\\ (2)\ & \Rightarrow p(y|x;\theta)=(h_\theta(x))^y(1-h_\theta(x))^{1-y} \\ (3)\ & \Rightarrow M(\theta)=\prod_{i=1}^{m}p(y^{(i)}|x^{(i)};\theta) \\ (4)\ & \Rightarrow M(\theta)=\prod_{i=1}^{m}(h_\theta(x^{(i)}))^y^{(i)}(1-h_\theta(x^{(i)}))^{1-y^{(i)}}\\ (5)\ & \Rightarrow log(M(\theta))=\sum_{i=1}^{m}[y^{(i)}log(h_\theta(x^{(i)})) +(1-y^{(i)})log(1-h_\theta(x^{(i)}))] \\ (6)\ & \Rightarrow L(\theta)=-log(M(\theta))=-\sum_{i=1}^{m}[y^{(i)}log(h_\theta(x^{(i)})) +(1-y^{(i)})log(1-h_\theta(x^{(i)}))] \end{aligned}